Drop world indexing from SPath

src/MicroSail/Symbolic/Mutator.v
@@ -756,31 +756,31 @@ Module Mutators
 
   Module SPath.
 
-    Inductive SPath (w : World) : Type :=
-    | angelic_binary (o1 o2 : SPath w)
-    | demonic_binary (o1 o2 : SPath w)
-    | error (msg : Message w)
+    Inductive SPath (Σ : LCtx) : Type :=
+    | angelic_binary (o1 o2 : SPath Σ)
+    | demonic_binary (o1 o2 : SPath Σ)
+    | error (msg : Message Σ)
     | block
-    | assertk (fml : Formula w) (msg : Message w) (k : SPath (wformula w fml))
-    | assumek (fml : Formula w) (k : SPath (wformula w fml))
+    | assertk (fml : Formula Σ) (msg : Message Σ) (k : SPath Σ)
+    | assumek (fml : Formula Σ) (k : SPath Σ)
     (* Don't use these two directly. Instead, use the HOAS versions 'angelic' *)
     (* and 'demonic' that will freshen names. *)
-    | angelicv b (k : SPath (wsnoc w b))
-    | demonicv b (k : SPath (wsnoc w b))
+    | angelicv b (k : SPath (Σ ▻ b))
+    | demonicv b (k : SPath (Σ ▻ b))
     | assert_vareq
-        x σ (xIn : x::σ ∈ w)
-        (t : Term (w - (x::σ)) σ)
-        (msg : Message (w - (x::σ)))
-        (k : SPath (wsubst w x t))
+        x σ (xIn : x::σ ∈ Σ)
+        (t : Term (Σ - (x::σ)) σ)
+        (msg : Message (Σ - (x::σ)))
+        (k : SPath (Σ - (x::σ)))
     | assume_vareq
-        x σ (xIn : (x,σ) ∈ w)
-        (t : Term (w - (x,σ)) σ)
-        (k : SPath (wsubst w x t))
+        x σ (xIn : (x,σ) ∈ Σ)
+        (t : Term (Σ - (x::σ)) σ)
+        (k : SPath (Σ - (x::σ)))
     | debug
         {BT B} {subB : Subst BT}
         {instB : Inst BT B}
         {occB: OccursCheck BT}
-        (b : BT w) (k : SPath w).
+        (b : BT Σ) (k : SPath Σ).
 
     Global Arguments error {_} _.
     Global Arguments block {_}.
@@ -792,35 +792,35 @@ Module Mutators
     Global Arguments assume_vareq {_} x {_ _} t k.
 
     Definition demonic_close :
-      forall Σ, SPath {| wctx := Σ; wco := nil |} -> SPath wnil :=
+      forall Σ, SPath Σ -> SPath wnil :=
       fix close Σ :=
         match Σ with
         | ctx_nil      => fun k => k
-        | ctx_snoc Σ b => fun k => close Σ (@demonicv (@MkWorld Σ []) b k)
+        | ctx_snoc Σ b => fun k => close Σ (@demonicv Σ b k)
         end.
 
     Global Instance persistent_spath : Persistent SPath :=
       (* ⊢ SPath -> □SPath := *)
-       fix pers {w0} p {w1} ω01 {struct p} : SPath w1 :=
+       fix pers (w0 : World) (p : SPath w0) {w1 : World} ω01 {struct p} : SPath w1 :=
          match p with
-         | angelic_binary p1 p2 => angelic_binary (pers p1 ω01) (pers p2 ω01)
-         | demonic_binary p1 p2 => demonic_binary (pers p1 ω01) (pers p2 ω01)
+         | angelic_binary p1 p2 => angelic_binary (pers w0 p1 ω01) (pers w0 p2 ω01)
+         | demonic_binary p1 p2 => demonic_binary (pers w0 p1 ω01) (pers w0 p2 ω01)
          | error msg            => error (subst msg (wsub ω01))
          | block                => block
          | assertk fml msg p0   =>
              assertk (subst fml (wsub ω01)) (subst msg (wsub ω01))
-               (pers p0 (wacc_formula ω01 fml))
+               (pers (wformula w0 fml) p0 (wacc_formula ω01 fml))
          | assumek fml p        =>
              assumek (subst fml (wsub ω01))
-               (pers p (wacc_formula ω01 fml))
-         | angelicv b p0        => angelicv b (pers p0 (wacc_snoc ω01 b))
-         | demonicv b p0        => demonicv b (pers p0 (wacc_snoc ω01 b))
+               (pers (wformula w0 fml) p (wacc_formula ω01 fml))
+         | angelicv b p0        => angelicv b (pers (wsnoc w0 b) p0 (wacc_snoc ω01 b))
+         | demonicv b p0        => demonicv b (pers (wsnoc w0 b) p0 (wacc_snoc ω01 b))
          | assert_vareq x t msg p =>
            let ζ := subst (sub_shift _) (wsub ω01) in
            assertk
              (formula_eq (env_lookup (wsub ω01) _) (subst t ζ))
              (subst msg ζ)
-             (pers p
+             (pers (wsubst w0 x t) p
                 (MkAcc (MkWorld (subst (wco w0) (sub_single _ t)))
                    (MkWorld
                       (cons (formula_eq (env_lookup (wsub ω01) _) (subst t ζ))
@@ -829,47 +829,39 @@ Module Mutators
            let ζ := subst (sub_shift _) (wsub ω01) in
            assumek
              (formula_eq (env_lookup (wsub ω01) _) (subst t ζ))
-             (pers p
+             (pers (wsubst w0 x t) p
                 (MkAcc (MkWorld (subst (wco w0) (sub_single _ t)))
                    (MkWorld
                       (cons (formula_eq (env_lookup (wsub ω01) _) (subst t ζ))
                          (wco w1))) ζ))
-         | debug d p => debug (subst d (wsub ω01)) (pers p ω01)
+         | debug d p => debug (subst d (wsub ω01)) (pers w0 p ω01)
          end.
 
-    Definition assume_formulas_without_solver {w : World} :
-      forall (fmls : List Formula w), SPath (wformulas w fmls) -> SPath w :=
-      match w with
-      | @MkWorld Σ pc =>
-        (fix assumes pc (fmls : List Formula Σ) {struct fmls} :
-           SPath {| wctx := Σ; wco := app fmls pc |} ->
-           SPath {| wctx := Σ; wco := pc |} :=
-           match fmls with
-           | nil => fun p => p
-           | cons fml fmls =>
-             fun p =>
-               assumes pc fmls
-                 (assumek (w:= {| wctx := Σ; wco := app fmls pc |}) fml p)
-           end) pc
+    Fixpoint assume_formulas_without_solver' {Σ}
+      (fmls : List Formula Σ) (p : SPath Σ) : SPath Σ :=
+      match fmls with
+      | nil           => p
+      | cons fml fmls => assume_formulas_without_solver' fmls (assumek fml p)
       end.
+
+    Fixpoint assert_formulas_without_solver' {Σ}
+      (msg : Message Σ) (fmls : List Formula Σ) (p : SPath Σ) : SPath Σ :=
+      match fmls with
+      | nil => p
+      | cons fml fmls =>
+        assert_formulas_without_solver' msg fmls (assertk fml msg p)
+      end.
+
+    (* These versions just add the world indexing. They simply enforces
+       that p should have been computed in the world with fmls added. *)
+    Definition assume_formulas_without_solver {w : World}
+      (fmls : List Formula w) (p : SPath (wformulas w fmls)) : SPath w :=
+      assume_formulas_without_solver' fmls p.
     Global Arguments assume_formulas_without_solver {_} fmls p.
 
-    Definition assert_formulas_without_solver {w : World} :
-      forall (msg : Message w) (fmls : List Formula w), SPath (wformulas w fmls) -> SPath w :=
-      match w with
-      | @MkWorld Σ pc =>
-        fun msg =>
-        (fix asserts pc (fmls : List Formula Σ) {struct fmls} :
-           SPath {| wctx := Σ; wco := app fmls pc |} ->
-           SPath {| wctx := Σ; wco := pc |} :=
-           match fmls with
-           | nil => fun p => p
-           | cons fml fmls =>
-             fun p =>
-               asserts pc fmls
-                 (assertk (w:= {| wctx := Σ; wco := app fmls pc |}) fml msg p)
-           end) pc
-      end.
+    Definition assert_formulas_without_solver {w : World} (msg : Message w)
+      (fmls : List Formula w) (p : SPath (wformulas w fmls)) : SPath w :=
+      assert_formulas_without_solver' msg fmls p.
     Global Arguments assert_formulas_without_solver {_} msg fmls p.
 
     Fixpoint assume_multisub {w1 w2} (ν : MultiSub w1 w2) :
@@ -878,9 +870,7 @@ Module Mutators
       destruct ν; intros o; cbn in o.
       - exact o.
       - apply (@assume_vareq w1 x σ xIn t).
-        eapply assume_multisub.
-        apply ν.
-        apply o.
+        eapply (assume_multisub _ _ ν o).
     Defined.
 
     Fixpoint assert_multisub {w1 w2} (msg : Message (wctx w1)) (ζ : MultiSub w1 w2) :
@@ -893,11 +883,9 @@ Module Mutators
         refine (assert_multisub (wsubst w1 x t) _ (subst msg (sub_single xIn t)) ζ o).
     Defined.
 
-    Definition safe :
-      (* ⊢ SPath AT -> SymInstance -> PROP := *)
-      forall w (o : SPath w) (ι : SymInstance w), Prop :=
-      fix safe {w} o ι :=
-        match o with
+    Fixpoint safe {Σ} (p : SPath Σ) (ι : SymInstance Σ) : Prop :=
+      (* ⊢ SPath -> SymInstance -> PROP := *)
+        match p with
         | angelic_binary o1 o2 => safe o1 ι \/ safe o2 ι
         | demonic_binary o1 o2 => safe o1 ι /\ safe o2 ι
         | error msg => False
@@ -918,7 +906,34 @@ Module Mutators
           safe k ι'
         | debug d k => Debug (inst d ι) (safe k ι)
         end%type.
-    Global Arguments safe {w} o ι.
+    Global Arguments safe {Σ} p ι.
+
+    (* We use a world indexed version of safe in the soundness proofs, just to make
+       Coq's unifier happy. *)
+    Fixpoint wsafe {w : World} (p : SPath w) (ι : SymInstance w) : Prop :=
+      (* ⊢ SPath -> SymInstance -> PROP := *)
+        match p with
+        | angelic_binary o1 o2 => wsafe o1 ι \/ wsafe o2 ι
+        | demonic_binary o1 o2 => wsafe o1 ι /\ wsafe o2 ι
+        | error msg => False
+        | block => True
+        | assertk fml msg o =>
+          Obligation msg fml ι /\ @wsafe (wformula w fml) o ι
+        | assumek fml o => (inst fml ι : Prop) -> @wsafe (wformula w fml) o ι
+        | angelicv b k => exists v, @wsafe (wsnoc w b) k (env_snoc ι b v)
+        | demonicv b k => forall v, @wsafe (wsnoc w b) k (env_snoc ι b v)
+        | @assert_vareq _ x σ xIn t msg k =>
+          (let ζ := sub_shift xIn in
+          Obligation (subst msg ζ) (formula_eq (term_var x) (subst t ζ))) ι /\
+          (let ι' := env_remove (x,σ) ι xIn in
+          @wsafe (wsubst w x t) k ι')
+        | @assume_vareq _ x σ xIn t k =>
+          let ι' := env_remove (x,σ) ι xIn in
+          env_lookup ι xIn = inst t ι' ->
+          @wsafe (wsubst w x t) k ι'
+        | debug d k => Debug (inst d ι) (wsafe k ι)
+        end%type.
+    Global Arguments wsafe {w} p ι.
 
     Lemma obligation_equiv {Σ : LCtx} (msg : Message Σ) (fml : Formula Σ) (ι : SymInstance Σ) :
       Obligation msg fml ι <-> inst fml ι.
@@ -928,56 +943,67 @@ Module Mutators
       @Debug B b P <-> P.
     Proof. split. now intros []. now constructor. Qed.
 
-    Lemma safe_persist  {w1 w2 : World} (ω12 : w1 ⊒ w2)
-          (o : SPath w1) (ι2 : SymInstance w2) :
-      safe (persist (A := SPath) o ω12) ι2 <->
-      safe o (inst (T := Sub _) ω12 ι2).
+    Lemma wsafe_safe {w : World} (p : SPath w) (ι : SymInstance w) :
+      wsafe p ι <-> safe p ι.
     Proof.
-      revert w2 ω12 ι2.
-      induction o; cbn; intros.
-      - now rewrite IHo1, IHo2.
-      - now rewrite IHo1, IHo2.
-      - split; intros [].
-      - reflexivity.
-      - rewrite ?obligation_equiv.
-        now rewrite IHo, inst_subst.
-      - now rewrite IHo, inst_subst.
-      - split; intros [v HYP]; exists v; revert HYP;
-          rewrite IHo; unfold wacc_snoc, wsnoc;
-            cbn [wctx wsub]; now rewrite inst_sub_up1.
-      - split; intros HYP v; specialize (HYP v); revert HYP;
-          rewrite IHo; unfold wacc_snoc, wsnoc;
-            cbn [wctx wsub]; now rewrite inst_sub_up1.
-      - rewrite ?obligation_equiv.
-        rewrite IHo; unfold wsubst; cbn [wctx wsub]. cbn.
-        now rewrite ?inst_subst, ?inst_sub_shift, <- inst_lookup.
-      - rewrite IHo; unfold wsubst; cbn [wctx wsub].
-        now rewrite ?inst_subst, ?inst_sub_shift, <- inst_lookup.
-      - now rewrite ?debug_equiv.
+      destruct w as [Σ pc]; cbn in *; revert pc.
+      induction p; cbn; intros pc; rewrite ?debug_equiv; auto;
+        try (intuition; fail).
+      apply base.exist_proper; eauto.
     Qed.
 
+    (* Lemma safe_persist  {w1 w2 : World} (ω12 : w1 ⊒ w2) *)
+    (*       (o : SPath w1) (ι2 : SymInstance w2) : *)
+    (*   safe (persist (A := SPath) o ω12) ι2 <-> *)
+    (*   safe o (inst (T := Sub _) ω12 ι2). *)
+    (* Proof. *)
+    (*   revert w2 ω12 ι2. *)
+    (*   induction o; cbn; intros. *)
+    (*   - now rewrite IHo1, IHo2. *)
+    (*   - now rewrite IHo1, IHo2. *)
+    (*   - split; intros []. *)
+    (*   - reflexivity. *)
+    (*   - rewrite ?obligation_equiv. *)
+    (*     now rewrite IHo, inst_subst. *)
+    (*   - now rewrite IHo, inst_subst. *)
+    (*   - split; intros [v HYP]; exists v; revert HYP; *)
+    (*       rewrite IHo; unfold wacc_snoc, wsnoc; *)
+    (*         cbn [wctx wsub]; now rewrite inst_sub_up1. *)
+    (*   - split; intros HYP v; specialize (HYP v); revert HYP; *)
+    (*       rewrite IHo; unfold wacc_snoc, wsnoc; *)
+    (*         cbn [wctx wsub]; now rewrite inst_sub_up1. *)
+    (*   - rewrite ?obligation_equiv. *)
+    (*     rewrite IHo; unfold wsubst; cbn [wctx wsub]. cbn. *)
+    (*     now rewrite ?inst_subst, ?inst_sub_shift, <- inst_lookup. *)
+    (*   - rewrite IHo; unfold wsubst; cbn [wctx wsub]. *)
+    (*     now rewrite ?inst_subst, ?inst_sub_shift, <- inst_lookup. *)
+    (*   - now rewrite ?debug_equiv. *)
+    (* Qed. *)
+
     Lemma safe_assume_formulas_without_solver {w0 : World}
-      (fmls : List Formula w0) (o : SPath (wformulas w0 fmls))
-      (ι0 : SymInstance w0) :
-      safe (assume_formulas_without_solver fmls o) ι0 <->
-      (instpc fmls ι0 -> safe o ι0).
+      (fmls : List Formula w0) (p : SPath w0) (ι0 : SymInstance w0) :
+      wsafe (assume_formulas_without_solver fmls p) ι0 <->
+      (instpc fmls ι0 -> @wsafe (wformulas w0 fmls) p ι0).
     Proof.
-      destruct w0. unfold assume_formulas_without_solver. cbn in fmls.
-      induction fmls; unfold wformulas; cbn in *.
-      - split; auto. intros HYP. apply HYP. constructor.
+      unfold assume_formulas_without_solver. revert p.
+      induction fmls; cbn in *; intros p.
+      - destruct w0; cbn; split; auto.
+        intros HYP. apply HYP. constructor.
       - rewrite IHfmls, inst_pathcondition_cons. cbn.
         intuition.
     Qed.
 
     Lemma safe_assert_formulas_without_solver {w0 : World}
-      (msg : Message w0) (fmls : List Formula w0) (o : SPath (wformulas w0 fmls))
+      (msg : Message w0) (fmls : List Formula w0) (p : SPath w0)
       (ι0 : SymInstance w0) :
-      safe (assert_formulas_without_solver msg fmls o) ι0 <->
-      (instpc fmls ι0 /\ safe o ι0).
+      wsafe (assert_formulas_without_solver msg fmls p) ι0 <->
+      (instpc fmls ι0 /\ @wsafe (wformulas w0 fmls) p ι0).
     Proof.
-      destruct w0. unfold assert_formulas_without_solver. cbn in fmls.
-      induction fmls; unfold wformulas; cbn in *.
-      - split. intros HYP. split; auto. constructor. intros []; auto.
+      unfold assert_formulas_without_solver. revert p.
+      induction fmls; cbn in *; intros p.
+      - destruct w0; cbn; split.
+        + intros HYP. split; auto. constructor.
+        + intros []; auto.
       - rewrite IHfmls, inst_pathcondition_cons; cbn.
         split; intros []; auto.
         + destruct H0. destruct H0. auto.
@@ -987,8 +1013,8 @@ Module Mutators
 
     Lemma safe_assume_multisub {w0 w1} (ζ : MultiSub w0 w1)
       (o : SPath w1) (ι0 : SymInstance w0) :
-      safe (assume_multisub ζ o) ι0 <->
-      (inst_multisub ζ ι0 -> safe o (inst (sub_multishift ζ) ι0)).
+      wsafe (assume_multisub ζ o) ι0 <->
+      (inst_multisub ζ ι0 -> wsafe o (inst (sub_multishift ζ) ι0)).
     Proof.
       induction ζ; cbn in *.
       - rewrite inst_sub_id. intuition.
@@ -1000,12 +1026,12 @@ Module Mutators
 
     Lemma safe_assert_multisub {w0 w1} msg (ζ : MultiSub w0 w1)
       (o : Message w1 -> SPath w1) (ι0 : SymInstance w0) :
-      safe (assert_multisub msg ζ o) ι0 <->
-      (inst_multisub ζ ι0 /\ safe (o (subst msg (wmultisub_sup ζ))) (inst (sub_multishift ζ) ι0)).
+      wsafe (assert_multisub msg ζ o) ι0 <->
+      (inst_multisub ζ ι0 /\ wsafe (o (subst msg (wmultisub_sup ζ))) (inst (sub_multishift ζ) ι0)).
     Proof.
       induction ζ.
       - cbn. rewrite inst_sub_id, subst_sub_id. intuition.
-      - cbn [safe assert_multisub inst_multisub
+      - cbn [wsafe assert_multisub inst_multisub
                   sub_multishift wmultisub_sup wtrans wsub].
         rewrite obligation_equiv.
         rewrite subst_sub_comp. cbn.
@@ -1015,113 +1041,149 @@ Module Mutators
         intuition.
     Qed.
 
-    Definition angelic_binary_prune :
-      ⊢ SPath -> SPath -> SPath :=
-      fun w o1 o2 =>
-        match o1 , o2 with
-        | block   , _       => block
-        | _       , block   => block
-        | error _ , _       => o2
-        | _       , error _ => o1
-        | _       , _       => angelic_binary o1 o2
-        end.
+    Fixpoint occurs_check_spath {Σ x} (xIn : x ∈ Σ) (p : SPath Σ) : option (SPath (Σ - x)) :=
+      match p with
+      | angelic_binary o1 o2 =>
+        option_ap (option_map (angelic_binary (Σ := Σ - x)) (occurs_check_spath xIn o1)) (occurs_check_spath xIn o2)
+      | demonic_binary o1 o2 =>
+        option_ap (option_map (demonic_binary (Σ := Σ - x)) (occurs_check_spath xIn o1)) (occurs_check_spath xIn o2)
+      | error msg => option_map error (occurs_check xIn msg)
+      | block => Some block
+      | assertk P msg o =>
+        option_ap (option_ap (option_map (assertk (Σ := Σ - x)) (occurs_check xIn P)) (occurs_check xIn msg)) (occurs_check_spath xIn o)
+      | assumek P o => option_ap (option_map (assumek (Σ := Σ - x)) (occurs_check xIn P)) (occurs_check_spath xIn o)
+      | angelicv b o => option_map (angelicv b) (occurs_check_spath (inctx_succ xIn) o)
+      | demonicv b o => option_map (demonicv b) (occurs_check_spath (inctx_succ xIn) o)
+      | @assert_vareq _ y σ yIn t msg o =>
+        match occurs_check_view yIn xIn with
+        | Same _ => None
+        | @Diff _ _ _ _ x xIn =>
+          option_ap
+            (option_ap
+               (option_map
+                  (fun (t' : Term (Σ - (y :: σ) - x) σ) (msg' : Message (Σ - (y :: σ) - x)) (o' : SPath (Σ - (y :: σ) - x)) =>
+                     let e := swap_remove yIn xIn in
+                     assert_vareq
+                       y
+                       (eq_rect (Σ - (y :: σ) - x) (fun Σ => Term Σ σ) t' (Σ - x - (y :: σ)) e)
+                       (eq_rect (Σ - (y :: σ) - x) Message msg' (Σ - x - (y :: σ)) e)
+                       (eq_rect (Σ - (y :: σ) - x) SPath o' (Σ - x - (y :: σ)) e))
+                  (occurs_check xIn t))
+               (occurs_check xIn msg))
+            (occurs_check_spath xIn o)
+        end
+      | @assume_vareq _ y σ yIn t o =>
+        match occurs_check_view yIn xIn with
+        | Same _ => Some o
+        | @Diff _ _ _ _ x xIn =>
+          option_ap
+            (option_map
+               (fun (t' : Term (Σ - (y :: σ) - x) σ) (o' : SPath (Σ - (y :: σ) - x)) =>
+                  let e := swap_remove yIn xIn in
+                  assume_vareq
+                    y
+                    (eq_rect (Σ - (y :: σ) - x) (fun Σ => Term Σ σ) t' (Σ - x - (y :: σ)) e)
+                    (eq_rect (Σ - (y :: σ) - x) SPath o' (Σ - x - (y :: σ)) e))
+               (occurs_check xIn t))
+            (occurs_check_spath xIn o)
+        end
+      | debug b o => option_ap (option_map (debug (Σ := Σ - x)) (occurs_check xIn b)) (occurs_check_spath xIn o)
+      end.
 
-    Definition demonic_binary_prune :
-      ⊢ SPath -> SPath -> SPath :=
-      fun w o1 o2 =>
-        match o1 , o2 with
-        | block   , _       => o2
-        | _       , block   => o1
-        | error s , _       => error s
-        | _       , error s => error s
-        | _       , _       => demonic_binary o1 o2
-        end.
+    Definition angelic_binary_prune {Σ} (p1 p2 : SPath Σ) : SPath Σ :=
+      match p1 , p2 with
+      | block   , _       => block
+      | _       , block   => block
+      | error _ , _       => p2
+      | _       , error _ => p1
+      | _       , _       => angelic_binary p1 p2
+      end.
 
-    Definition assertk_prune :
-      (* ⊢ Formula -> Message -> SPath AT -> SPath AT. *)
-      forall {w : World} (fml : Formula w), Message w -> SPath (wformula w fml) -> SPath w :=
-      fun w fml msg o =>
-        match o with
-        | error s => @error w s
-        | _       => assertk fml msg o
-        end.
-    Global Arguments assertk_prune {w} fml msg p.
+    Definition demonic_binary_prune {Σ} (p1 p2 : SPath Σ) : SPath Σ :=
+      match p1 , p2 with
+      | block   , _       => p2
+      | _       , block   => p1
+      | error s , _       => error s
+      | _       , error s => error s
+      | _       , _       => demonic_binary p1 p2
+      end.
 
-    Definition assumek_prune :
-      (* ⊢ Formula -> SPath AT -> SPath AT := *)
-      forall {w : World} (fml : Formula w), SPath (wformula w fml) -> SPath w :=
-      fun w fml o =>
-        match o with
-        | block => block
-        | _     => assumek fml o
-        end.
-    Global Arguments assumek_prune {w} fml p.
+    Definition assertk_prune {Σ} (fml : Formula Σ) (msg : Message Σ) (p : SPath Σ) : SPath Σ :=
+      match p with
+      | error s => @error Σ s
+      | _       => assertk fml msg p
+      end.
+    Global Arguments assertk_prune {Σ} fml msg p.
 
-    Definition angelicv_prune b :
-      ⊢ Snoc (SPath) b -> SPath :=
-      fun w o => angelicv b o.
-        (* This is not good *)
-        (* match o with *)
-        (* | error s => error s *)
-        (* | _           => angelicv b o *)
-        (* end. *)
+    Definition assumek_prune {Σ} (fml : Formula Σ) (p : SPath Σ) : SPath Σ :=
+      match p with
+      | block => block
+      | _     => assumek fml p
+      end.
+    Global Arguments assumek_prune {Σ} fml p.
 
-    Definition demonicv_prune b :
-      ⊢ Snoc SPath b -> SPath :=
-      fun w o =>
-        (* match @occurs_check_spath AT _ (Σ ▻ b) b inctx_zero o with *)
-        (* | Some o => o *)
-        (* | None   => demonicv b o *)
-        (* end. *)
-        match o with
-        | block => block
-        | _  => demonicv b o
-        end.
+    Definition angelicv_prune {Σ} b (p : SPath (Σ ▻ b)) : SPath Σ :=
+      angelicv b p.
+      (* TODO: This does not work because of the message that is included in *)
+      (* the error. We should make it possible to "strengthen" the message by *)
+      (* adding a constructor: Message (Σ ▻ b) -> Message Σ. *)
+      (* match p with *)
+      (* | error s => error s *)
+      (* | _       => angelicv b p *)
+      (* end. *)
 
-    Definition assume_vareq_prune {w}
-      {x σ} {xIn : (x,σ) ∈ wctx w} (t : Term (w - (x,σ)) σ) (k : SPath (wsubst w x t)) : SPath w :=
+    Definition demonicv_prune {Σ} b (p : SPath (Σ ▻ b)) : SPath Σ :=
+      (* match @occurs_check_spath AT _ (Σ ▻ b) b inctx_zero o with *)
+      (* | Some o => o *)
+      (* | None   => demonicv b o *)
+      (* end. *)
+      match p with
+      | block => block
+      | _     => demonicv b p
+      end.
+
+    Definition assume_vareq_prune {Σ} {x σ} {xIn : x::σ ∈ Σ}
+      (t : Term (Σ - (x::σ)) σ) (k : SPath (Σ - (x::σ))) : SPath Σ :=
       match k with
       | block => block
-      | _          => assume_vareq x t k
+      | _     => assume_vareq x t k
       end.
-    Global Arguments assume_vareq_prune {w} x {σ xIn} t k.
+    Global Arguments assume_vareq_prune {Σ} x {σ xIn} t k.
 
-    Definition assert_vareq_prune {w}
-      {x σ} {xIn : (x,σ) ∈ wctx w} (t : Term (w - (x,σ)) σ)
-      (msg : Message (w - (x,σ))) (k : SPath (wsubst w x t)) : SPath w :=
+    Definition assert_vareq_prune {Σ} {x σ} {xIn : x::σ ∈ Σ}
+      (t : Term (Σ - (x::σ)) σ) (msg : Message (Σ - (x::σ))) (k : SPath (Σ - (x::σ))) : SPath Σ :=
       match k with
-      (* | fail s => fail s *)
+      (* TODO: Like for angelicv *)
+      (* | error s => error s *)
       | _          => assert_vareq x t msg k
       end.
-    Global Arguments assert_vareq_prune {w} x {σ xIn} t msg k.
+    Global Arguments assert_vareq_prune {Σ} x {σ xIn} t msg k.
 
-    Definition prune :
-      ⊢ SPath -> SPath :=
-      fix prune {w} o :=
-        match o with
-        | error msg => error msg
-        | block => block
-        | angelic_binary o1 o2 =>
-          angelic_binary_prune (prune o1) (prune o2)
-        | demonic_binary o1 o2 =>
-          demonic_binary_prune (prune o1) (prune o2)
-        | assertk fml msg o =>
-          assertk_prune fml msg (prune o)
-        | assumek fml o =>
-          assumek_prune fml (prune o)
-        | angelicv b o =>
-          angelicv_prune (prune o)
-        | demonicv b o =>
-          demonicv_prune (prune o)
-        | assert_vareq x t msg k =>
-          assert_vareq_prune x t msg (prune k)
-        | assume_vareq x t k =>
-          assume_vareq_prune x t (prune k)
-        | debug d k =>
-          debug d (prune k)
-        end.
+    Fixpoint prune {Σ} (p : SPath Σ) : SPath Σ :=
+      match p with
+      | error msg => error msg
+      | block => block
+      | angelic_binary o1 o2 =>
+        angelic_binary_prune (prune o1) (prune o2)
+      | demonic_binary o1 o2 =>
+        demonic_binary_prune (prune o1) (prune o2)
+      | assertk fml msg o =>
+        assertk_prune fml msg (prune o)
+      | assumek fml o =>
+        assumek_prune fml (prune o)
+      | angelicv b o =>
+        angelicv_prune (prune o)
+      | demonicv b o =>
+        demonicv_prune (prune o)
+      | assert_vareq x t msg k =>
+        assert_vareq_prune x t msg (prune k)
+      | assume_vareq x t k =>
+        assume_vareq_prune x t (prune k)
+      | debug d k =>
+        debug d (prune k)
+      end.
 
-    Lemma prune_angelic_binary_sound {w} (p1 p2 : SPath w) (ι : SymInstance w) :
+    Lemma prune_angelic_binary_sound {Σ} (p1 p2 : SPath Σ) (ι : SymInstance Σ) :
       safe (angelic_binary_prune p1 p2) ι <-> safe (angelic_binary p1 p2) ι.
     Proof.
       destruct p1; cbn; auto.
@@ -1140,7 +1202,7 @@ Module Mutators
       - destruct p2; cbn; auto; intuition.
     Qed.
 
-    Lemma prune_demonic_binary_sound {w} (p1 p2 : SPath w) (ι : SymInstance w) :
+    Lemma prune_demonic_binary_sound {Σ} (p1 p2 : SPath Σ) (ι : SymInstance Σ) :
       safe (demonic_binary_prune p1 p2) ι <-> safe (demonic_binary p1 p2) ι.
     Proof.
       destruct p1; cbn; auto.
@@ -1159,33 +1221,33 @@ Module Mutators
       - destruct p2; cbn; auto; intuition.
     Qed.
 
-    Lemma prune_assertk_sound {w} fml msg (p : SPath (wformula w fml)) (ι : SymInstance w) :
+    Lemma prune_assertk_sound {Σ} fml msg (p : SPath Σ) (ι : SymInstance Σ) :
       safe (assertk_prune fml msg p) ι <-> safe (assertk fml msg p) ι.
     Proof. destruct p; cbn; rewrite ?obligation_equiv; auto; intuition. Qed.
 
-    Lemma prune_assumek_sound {w} fml (p : SPath (wformula w fml)) (ι : SymInstance w) :
+    Lemma prune_assumek_sound {Σ} fml (p : SPath Σ) (ι : SymInstance Σ) :
       safe (assumek_prune fml p) ι <-> safe (assumek fml p) ι.
     Proof. destruct p; cbn; auto; intuition. Qed.
 
-    Lemma prune_angelicv_sound {w b} (p : SPath (wsnoc w b)) (ι : SymInstance w) :
+    Lemma prune_angelicv_sound {Σ b} (p : SPath (Σ ▻ b)) (ι : SymInstance Σ) :
       safe (angelicv_prune p) ι <-> safe (angelicv b p) ι.
     Proof. reflexivity. Qed.
 
-    Lemma prune_demonicv_sound {w b} (p : SPath (wsnoc w b)) (ι : SymInstance w) :
+    Lemma prune_demonicv_sound {Σ b} (p : SPath (Σ ▻ b)) (ι : SymInstance Σ) :
       safe (demonicv_prune p) ι <-> safe (demonicv b p) ι.
     Proof. destruct p; cbn; auto; intuition. Qed.
 
-    Lemma prune_assert_vareq_sound {w : World} {x σ} {xIn : x :: σ ∈ w}
-      (t : Term (w - (x :: σ)) σ) (msg : Message (w - (x :: σ))) (p : SPath (wsubst w x t)) (ι : SymInstance w) :
+    Lemma prune_assert_vareq_sound {Σ x σ} {xIn : x::σ ∈ Σ}
+      (t : Term (Σ - (x::σ)) σ) (msg : Message (Σ - (x::σ))) (p : SPath (Σ - (x::σ))) (ι : SymInstance Σ) :
       safe (assert_vareq_prune x t msg p) ι <-> safe (assert_vareq x t msg p) ι.
     Proof. reflexivity. Qed.
 
-    Lemma prune_assume_vareq_sound {w : World} {x σ} {xIn : x :: σ ∈ w}
-      (t : Term (w - (x :: σ)) σ) (p : SPath (wsubst w x t)) (ι : SymInstance w) :
+    Lemma prune_assume_vareq_sound {Σ x σ} {xIn : x::σ ∈ Σ}
+      (t : Term (Σ - (x::σ)) σ) (p : SPath (Σ - (x::σ))) (ι : SymInstance Σ) :
       safe (assume_vareq_prune x t p) ι <-> safe (assume_vareq x t p) ι.
     Proof. destruct p; cbn; auto; intuition. Qed.
 
-    Lemma prune_sound {w} (p : SPath w) (ι : SymInstance w) :
+    Lemma prune_sound {Σ} (p : SPath Σ) (ι : SymInstance Σ) :
       safe (prune p) ι <-> safe p ι.
     Proof.
       induction p; cbn [prune safe].
@@ -1298,6 +1360,12 @@ Module Mutators
           (* Assume variable equalities and the residual constraints *)
           assume_multisub ν
             (assume_formulas_without_solver fmls
+               (* Run POST in the world with the variable and residual
+                  formulas included. This is a critical piece of code since
+                  this is the place where we really meaningfully change the
+                  world. We changed the type of assume_formulas_without_solver
+                  just to not forget adding the formulas to the path constraints.
+               *)
                (four POST (wmultisub_sup ν) (wformulas_sup w1 fmls) tt))
         | None =>
           (* The formula is inconsistent with the path constraints. *)
@@ -1305,23 +1373,20 @@ Module Mutators
         end.
 
     Definition assert_formula :
-      ⊢ Message -> Formula -> SDijkstra Unit.
-      refine (
+      ⊢ Message -> Formula -> SDijkstra Unit :=
       fun w0 msg fml POST =>
         match solver fml with
         | Some (existT w1 (ν , fmls)) =>
           (* Assert variable equalities and the residual constraints *)
           assert_multisub msg ν
-            (fun msg' => assert_formulas_without_solver msg' fmls _)
+            (fun msg' =>
+               assert_formulas_without_solver msg' fmls
+                 (* Critical code. Like for assume_formula. *)
+                 (four POST (wmultisub_sup ν) (wformulas_sup w1 fmls) tt))
         | None =>
           (* The formula is inconsistent. *)
           error msg
-        end).
-      eapply (four POST); eauto.
-      apply (wmultisub_sup ν).
-      apply (wformulas_sup w1 fmls).
-      constructor.
-    Defined.
+        end.
 
     Definition assume_formulas :
       ⊢ List Formula -> SDijkstra Unit.
